

Sheet

[1] Differentiate the following functions:

$$1) y = \frac{1 + x - 4\sqrt{x}}{x}$$

$$2) y = (x^2 + 1)^2 \left(x + 5 + \frac{1}{x} \right)^3$$

$$3) y = \sqrt[7]{x^2} - x^3 + 8$$

$$4) y = e^{\sin^{-1} x}$$

$$5) y = \tan^2 x + x \cos^3 x$$

$$6) y = e^{\sqrt{x+1}} \ln(\tan x)$$

$$7) y = 10^x \log x$$

$$8) y = (\sec^{-1} x^4)^3$$

$$9) y = \cos^{-1} \left(\frac{a + b \cos x}{b + a \cos x} \right)$$

$$10) y = \tan^{-1} \sqrt{\frac{1 - \cos x}{1 + \cos x}}$$

$$11) y = e^{\ln(\sin^{-1} x^2)}$$

$$12) y = \frac{x e^{\sin^{-1} x}}{\sqrt{1-x^2}}$$

$$13) y = \ln \left(x + \sqrt{x^2 + 1} \right)$$

$$14) y = x^3 \cosh(x^2) - \coth(x^{-1})$$

$$15) y = \tanh(x^2 + \sin x)$$

$$16) y = \operatorname{sech}^2 \left(\sqrt{\cos^2 x + 1} \right)$$

[2] Find $\frac{dy}{dx}$ for the following functions

$$1) y = (x)^{\sin x}$$

$$2) y = \frac{x^x \sin^3 x}{e^{\cot(3x)} (x^2+4)^7}$$

$$3) y = \frac{x^2 \sqrt[3]{7x-14}}{e^{\sin x} (25-x^2)^4}$$

$$4) y = \frac{(x-1)^3 (1-\tan x)^4}{x^{\ln x} (2-\cos x)^2}$$

$$5) y = \sqrt[3]{\frac{x(x+5)e^x}{\sin^3 x}}$$

$$6) \sqrt{y} = \ln \left(\frac{\tan^{-1} 3x}{(x+1)^2 \cosh x} \right)$$

[3] Find the first derivative for the following functions

$$1) x^{\sin x} \cdot y = (\sin x)^x$$

$$2) x^y = \sin(x^3 + e^{7x^2})$$

$$3) y = \log_7 \left(\frac{\sin x \cos x}{e^{2x} 2^x} \right)^5$$

$$4) y = x[\log_5(x^2 - 2x)]^3$$

$$5) y = x^{\sin x} \cdot \cot^4(\sqrt{1-x^2})$$

$$6) y = \frac{x^x (2 - \cot^{-1} x)^{x^2}}{x^{\cos x} (1 - 2 \ln x)^5}.$$

[4] Find $\frac{dy}{dx}$ by implicit differentiation

1) $\log_3(\sqrt{x^3 + y^3}) + \sec^4(x^2 y^3) = 2$

2) $y^2 + 1 + xy = e^{xy}$

3) $e^{x^2 y} = 2x + 2y$

4) $x \tan^{-1} y = y \tan^{-1} x$

[5] Find $\frac{d^2 y}{dx^2}$ for the parametric functions

1) $x = \sqrt{1 - t^6}$, $y = \sin^{-1}(t^3)$

2) $x = \ln(1 + t^2)$, $y = \tan^{-1}(t)$

3) $x = \sin(\ln t)$, $y = \ln(\sin t)$

4) $x = \cos \theta + \theta \sin \theta$, $y = \sin \theta - \theta \cos \theta$

[6] If $y = x \sin \frac{1}{x}$. Prove that $x^4 y'' + y = 0$

[7] If $x = \sec^2(t^2 + 1)$, $y = \cos(t^2 + 1)$. Prove that $y'' = \frac{6}{x^4}$.

[8] If $x = \tan\left(\frac{\sqrt{t}}{t^2+1}\right)$, $y = \sec\left(\frac{\sqrt{t}}{t^2+1}\right)$. Show that $y'' = y^{-3}$.

[9] If $x = 2(1 - \cos \theta)$, $y = 2 \sin^2 \theta$. Show that $y'' = 1$.

Good Luck 